WIP call option

ContractExamples/FStar/NewCallOptionElaborated.fst
@@ -21,6 +21,14 @@ let price : U64.t = 100uL
 
 type pointedOutput = outpoint * output
 
+val tryAddPoint : outpoint -> utxos:utxo -> cost (result pointedOutput) 7
+let tryAddPoint pt utxos =
+  let open ET in
+  Zen.Cost.inc (match utxos pt with
+      | Some oput -> ret (pt, oput)
+      | None -> failw "Cannot find output in UTXO set")
+    7
+
 val tryAddPoints :
   #l:nat -> V.t outpoint l -> utxos:utxo -> cost (result (V.t pointedOutput l)) M.(20 * l + 20)
 let rec tryAddPoints #l v utxos =
@@ -44,15 +52,47 @@ type command =
   | Buy : V.t pointedOutput 2 -> outputLock -> command
   | Exercise : V.t pointedOutput 2 -> outputLock -> command
 
-val makeCommand : inputMsg -> cost (result command) 18
+
+
+
+
+
+  (*val makeCommand : inputMsg -> cost (result command) 33
+  let makeCommand imsg =
+    let d : cost (n:nat & inputData n) 3 = Zen.Cost.inc (ret @ imsg.data) 3 in
+    Zen.Cost.inc (do (| n , iData |) <-- d ;
+        do cmd <-- ret @ imsg.cmd ;
+        do utxos <-- ret @ imsg.utxo ;
+        let open M in
+        let open ET in
+        Zen.Cost.inc (match cmd, n with
+            | 0uy, 1 ->
+              begin match iData with
+                | Outpoint pt -> do pointed <-- tryAddPoint pt utxos ; ret @ Initialize pointed
+                | _ -> (inc (failw "Bad Initialization data") 7) <: (cost (result command) 7) end
+            | _ ->
+              let failure : cost (result command) 1 = Zen.Cost.inc (failw "Not implemented") 1 in
+              (Zen.Cost.inc (inc failure 4) 2) <: (cost (result command) 7))
+          14)
+      9*)
+
+
+
+
+
+val makeCommand : inputMsg -> cost (result command) 33
 let makeCommand imsg =
-  Zen.Cost.inc (do cmd <-- ret @ imsg.cmd ;
-      do d <-- ret @ imsg.data ;
+  let d : cost (n:nat & inputData n) 3 = Zen.Cost.inc (ret @ imsg.data) 3 in
+  Zen.Cost.inc (do (| n , iData |) <-- d ;
+      do cmd <-- ret @ imsg.cmd ;
+      do utxos <-- ret @ imsg.utxo ;
+      let open M in
       let open ET in
-      Zen.Cost.inc (match cmd, d with
-          | 0uy, _ -> failw "One"
-          | 1uy, _ -> failw "Two"
-          | 2uy, _ -> failw "Three"
-          | _ -> failw "Bad or unknown command")
-        10)
-    8
+      Zen.Cost.inc (match cmd, n with
+          | 0uy, 1 ->
+            begin match iData with
+              | Outpoint pt -> do pointed <-- tryAddPoint pt utxos ; ret @ Initialize pointed
+              | _ -> inc (failw "Bad Initialization data") 7  <: (cost (result command) 7) end
+          | _ -> inc (failw "Not implemented") 7  <: (cost (result command) 7))
+        14)
+    9
